Move some non-rc11 specific definitions to exec

exec.v
@@ -1157,3 +1157,481 @@ that was written at some point *)
 
 Definition complete_exec (e: Execution) :=
   valid_exec e /\ Included _ (reads (evts e)) (ran e.(rf)).
+
+Section Derived.
+
+Variable ex: Execution.
+
+(** * Derived relations *)
+
+(** ** Reads-before *)
+
+(** A read event [r] reads-before a write event [w] if it reads-from a write
+event sequenced before [w] by the modification order. It corresponds to the
+from-read relation in some other works on axiomatic memory models. *)
+
+Definition rb :=
+  (rf ex) ° ⋅ (mo ex).
+
+Lemma rf_wr:
+  valid_exec ex ->
+  (rf ex) ≡ [W] ⋅ (rf ex) ⋅ [R].
+Proof.
+  intros Hval.
+  destruct_val_exec Hval.
+  destruct Hrf_v as [_ [_ [Hwr _]]].
+  fold rf in Hwr. rewrite Hwr. unfold rf; intuition.
+Qed.
+
+Lemma mo_ww:
+  valid_exec ex ->
+  (mo ex) ≡ [W] ⋅ (mo ex) ⋅ [W].
+Proof.
+  intros Hval.
+  destruct_val_exec Hval.
+  destruct Hmo_v as [Hmo _].
+  fold mo in Hmo. rewrite Hmo. unfold mo; intuition.
+Qed.
+
+Lemma rb_rw:
+  valid_exec ex ->
+  rb ≡ [R] ⋅ rb ⋅ [W].
+Proof.
+  intros Hval.
+  unfold rb.
+  rewrite (mo_ww Hval).
+  rewrite (rf_wr Hval).
+  ra_normalise.
+  rewrite 2injcnv.
+  kat.
+Qed.
+
+(** In a valid execution, the sequenced-before relation is irreflexive *)
+
+Lemma sb_irr:
+  valid_exec ex ->
+  irreflexive (sb ex).
+Proof.
+  intros Hval.
+  apply irreflexive_is_irreflexive.
+  destruct_val_exec Hval.
+  destruct_sb_v Hsb_v.
+  destruct Hsb_lso as [_ [_ Hsbirr]].
+  intros x. apply Hsbirr.
+Qed.
+
+(** In a valid execution, the read-from relation is irreflexive *)
+
+Lemma rf_irr:
+  valid_exec ex ->
+  irreflexive (rf ex).
+Proof.
+  intros Hval.
+  unfold irreflexive.
+  rewrite (rf_wr Hval), refl_double, capone.
+  mrewrite rw_0. ra.
+Qed.
+
+(** In a valid execution, the modification order is irreflexive *)
+
+Lemma mo_irr:
+  valid_exec ex ->
+  irreflexive (mo ex).
+Proof.
+  intros Hval.
+  apply irreflexive_is_irreflexive.
+  intros x Hnot.
+  destruct_val_exec Hval.
+  destruct_mo_v Hmo_v.
+  destruct Hmopo as [_ [_ ?]].
+  apply (H x). auto.
+Qed.
+
+(** In a valid execution, the reads-before relation is irreflexive *)
+
+Lemma rb_irr:
+  valid_exec ex ->
+  irreflexive rb.
+Proof.
+  intros Hval.
+  unfold irreflexive.
+  rewrite (rb_rw Hval), refl_double, capone.
+  mrewrite wr_0. ra.
+Qed.
+
+
+(** In a valid_execution, two events related by read-before belong to the set of
+events of the execution *)
+
+Lemma rb_orig_evts (x y : Event):
+  valid_exec ex ->
+  rb x y ->
+  In _ (evts ex) x.
+Proof.
+  intros Hval Hrb.
+  destruct Hrb as [z Hrf Hmo].
+  simp_cnv Hrf.
+  eapply rf_dest_evts; eauto using Hval.
+Qed.
+
+Lemma rb_dest_evts (x y : Event):
+  valid_exec ex ->
+  rb x y ->
+  In _ (evts ex) y.
+Proof.
+  intros Hval Hrb.
+  destruct Hrb as [z Hrf Hmo].
+  eapply mo_dest_evts; eauto using Hval.
+Qed.
+
+(** In a valid execution, an event in the origin of read-before is a read
+event *)
+
+Lemma rb_orig_read (x y : Event):
+  valid_exec ex ->
+  rb x y ->
+  is_read x.
+Proof.
+  intros Hval Hrb.
+  destruct Hrb as [z Hrf Hmo].
+  simp_cnv Hrf.
+  eapply rf_dest_read; eauto using Hval.
+Qed.
+
+(** In a valid execution, an event in the destination of read-before is a
+write event *)
+
+Lemma rb_dest_write (x y : Event):
+  valid_exec ex ->
+  rb x y ->
+  is_write y.
+Proof.
+  intros Hval Hrb.
+  destruct Hrb as [z Hrf Hmo].
+  eapply mo_dest_write; eauto using Hval.
+Qed.
+
+(** In a valid execution, two events related by read-before affect the same
+location *)
+
+Lemma rb_same_loc (x y : Event):
+  valid_exec ex ->
+  rb x y ->
+  (get_loc x) = (get_loc y).
+Proof.
+  intros Hval Hrb.
+  destruct Hrb as [z Hrf Hmo].
+  simp_cnv Hrf.
+  apply rf_same_loc in Hrf.
+  apply mo_same_loc in Hmo.
+  congruence.
+  all: eauto using Hval.
+Qed.
+
+(** In a valid execution, two events related by read-before are different *)
+
+Lemma rb_diff (x y : Event):
+  valid_exec ex ->
+  rb x y ->
+  x <> y.
+Proof.
+  intros Hval Hrb Heq.
+  eapply rb_irr. auto.
+  split; eauto.
+Qed.
+
+(** In a valid execution, reads-before is acyclic *)
+
+Lemma rb_ac:
+  valid_exec ex ->
+  acyclic rb.
+Proof.
+  intros Hval x Hcyc.
+  rewrite tc_inv_dcmp2 in Hcyc.
+  destruct Hcyc as [y Hfirst Hcyc].
+  rewrite rtc_inv_dcmp6 in Hcyc.
+  destruct Hcyc as [Hcyc|Hcyc].
+  { simpl in Hcyc. rewrite Hcyc in Hfirst.
+    eapply (rb_irr Hval x x); try (split; simpl); intuition eauto. }
+  rewrite tc_inv_dcmp2 in Hcyc.
+  destruct Hcyc as [z Hsecond Hcyc].
+  rewrite (rb_rw Hval) in Hfirst, Hsecond.
+  apply simpl_trt_tright in Hfirst.
+  apply simpl_trt_tleft in Hsecond.
+  destruct y; intuition auto.
+Qed.
+
+(** In a valid execution the union of modification-order and reads-before is
+acyclic *)
+
+Lemma rbmo_ac:
+  valid_exec ex ->
+  acyclic (rb ⊔ (mo ex)).
+Proof.
+  intros Hval x Hcyc.
+  rewrite union_comm in Hcyc.
+  unshelve (eapply (cyc_u_of_ac_implies_cyc_seq _ _ _ _ _ _) in Hcyc).
+  - unfold acyclic. apply mo_ac. eauto.
+  - intros z1 z2 [z3 H1 H2].
+    eapply mo_trans; eauto.
+  - apply rb_ac. auto.
+  - destruct Hcyc as [y Hcyc].
+    rewrite tc_inv_dcmp2 in Hcyc.
+    destruct Hcyc as [z1 [z2 Hmo Hrb] _].
+    rewrite tc_inv_dcmp2 in Hrb.
+    destruct Hrb as [z3 Hrb _].
+    rewrite (rb_rw Hval) in Hrb.
+    apply (mo_ww Hval) in Hmo.
+    apply simpl_trt_tright in Hmo.
+    apply simpl_trt_tleft in Hrb.
+    destruct z2; simpl in Hmo, Hrb; intuition auto.
+Qed.
+
+
+(** In a valid execution, the union of sequenced-before, reads-from, 
+modification order and reads-before is irreflexive *)
+
+Lemma sbrfmorb_irr:
+  valid_exec ex ->
+  irreflexive (sb ex ⊔ rf ex ⊔ mo ex ⊔ rb).
+Proof.
+  intros Hval.
+  apply irreflexive_union.
+  apply irreflexive_union.
+  apply irreflexive_union.
+  apply (sb_irr Hval).
+  apply (rf_irr Hval).
+  apply (mo_irr Hval).
+  apply (rb_irr Hval).
+Qed.
+
+Lemma sbrf_irr:
+  valid_exec ex ->
+  irreflexive (sb ex ⊔ rf ex).
+Proof.
+  intros Hval.
+  apply irreflexive_union.
+  - auto using sb_irr.
+  - auto using rf_irr.
+Qed.
+
+Lemma rtc_sbrfmorb_in_l_aux (x y: Event):
+  valid_exec ex ->
+  (sb ex ⊔ rf ex ⊔ mo ex ⊔ rb)^* x y ->
+  (fun z1 z2 => In _ (evts ex) z2 -> In _ (evts ex) z1) x y.
+Proof.
+  intros Hval.
+  apply rtc_ind.
+  - intros z1 z2 [[[Hsb|Hrf]|Hmo]|Hrb]; intros Hin.
+    * eapply sb_orig_evts; eauto.
+    * eapply rf_orig_evts; eauto.
+    * eapply mo_orig_evts; eauto.
+    * eapply rb_orig_evts; eauto.
+  - intuition auto.
+  - intuition auto.
+Qed.
+
+Lemma rtc_sbrfmorb_in_l (x y: Event):
+  valid_exec ex ->
+  (sb ex ⊔ rf ex ⊔ mo ex ⊔ rb)^* x y ->
+  In _ (evts ex) y ->
+  In _ (evts ex) x.
+Proof.
+  intros Hval Hrel Hy. eapply rtc_sbrfmorb_in_l_aux; eauto.
+Qed.
+
+Lemma rtc_sbrfmorb_in_r_aux (x y: Event):
+  valid_exec ex ->
+  (sb ex ⊔ rf ex ⊔ mo ex ⊔ rb)^* x y ->
+  (fun z1 z2 => In _ (evts ex) z1 -> In _ (evts ex) z2) x y.
+Proof.
+  intros Hval.
+  apply rtc_ind.
+  - intros z1 z2 [[[Hsb|Hrf]|Hmo]|Hrb]; intros Hin.
+    * eapply sb_dest_evts; eauto.
+    * eapply rf_dest_evts; eauto.
+    * eapply mo_dest_evts; eauto.
+    * eapply rb_dest_evts; eauto.
+  - intuition auto.
+  - intuition auto.
+Qed.
+
+Lemma rtc_sbrfmorb_in_r (x y: Event):
+  valid_exec ex ->
+  (sb ex ⊔ rf ex ⊔ mo ex ⊔ rb)^* x y ->
+  In _ (evts ex) x ->
+  In _ (evts ex) y.
+Proof.
+  intros Hval Hrel Hy. eapply rtc_sbrfmorb_in_r_aux; eauto.
+Qed.
+
+Lemma tc_sbrfmorb_in_l_aux (x y: Event):
+  valid_exec ex ->
+  (sb ex ⊔ rf ex ⊔ mo ex ⊔ rb)^+ x y ->
+  (fun z1 z2 => In _ (evts ex) z1) x y.
+Proof.
+  intros Hval.
+  apply tc_ind.
+  - intros z1 z2 [[[Hsb|Hrf]|Hmo]|Hrb].
+    * eapply sb_orig_evts; eauto.
+    * eapply rf_orig_evts; eauto.
+    * eapply mo_orig_evts; eauto.
+    * eapply rb_orig_evts; eauto.
+  - intuition auto.
+Qed.
+
+Lemma tc_sbrfmorb_in_l (x y: Event):
+  valid_exec ex ->
+  (sb ex ⊔ rf ex ⊔ mo ex ⊔ rb)^+ x y ->
+  In _ (evts ex) x.
+Proof.
+  intros Hval Hrel. eapply tc_sbrfmorb_in_l_aux; eauto.
+Qed.
+
+Lemma tc_sbrfmorb_in_r_aux (x y: Event):
+  valid_exec ex ->
+  (sb ex ⊔ rf ex ⊔ mo ex ⊔ rb)^+ x y ->
+  (fun z1 z2 => In _ (evts ex) z2) x y.
+Proof.
+  intros Hval.
+  apply tc_ind.
+  - intros z1 z2 [[[Hsb|Hrf]|Hmo]|Hrb].
+    * eapply sb_dest_evts; eauto.
+    * eapply rf_dest_evts; eauto.
+    * eapply mo_dest_evts; eauto.
+    * eapply rb_dest_evts; eauto.
+  - intuition auto.
+Qed.
+
+Lemma tc_sbrfmorb_in_r (x y: Event):
+  valid_exec ex ->
+  (sb ex ⊔ rf ex ⊔ mo ex ⊔ rb)^+ x y ->
+  In _ (evts ex) y.
+Proof.
+  intros Hval Hrel. eapply tc_sbrfmorb_in_r_aux; eauto.
+Qed.
+
+Lemma sbrfmorb_in_l (x y: Event):
+  valid_exec ex ->
+  (sb ex ⊔ rf ex ⊔ mo ex ⊔ rb) x y ->
+  In _ (evts ex) x.
+Proof.
+  intros Hval Hrel.
+  destruct Hrel as [[[Hrel|Hrel]|Hrel]|Hrel].
+  - eapply sb_orig_evts in Hrel; eauto.
+  - eapply rf_orig_evts in Hrel; eauto.
+  - eapply mo_orig_evts in Hrel; eauto.
+  - eapply rb_orig_evts in Hrel; eauto.
+Qed.
+
+Lemma sbrfmorb_in_r (x y: Event):
+  valid_exec ex ->
+  (sb ex ⊔ rf ex ⊔ mo ex ⊔ rb) x y ->
+  In _ (evts ex) y.
+Proof.
+  intros Hval Hrel.
+  destruct Hrel as [[[Hrel|Hrel]|Hrel]|Hrel].
+  - eapply sb_dest_evts in Hrel; eauto.
+  - eapply rf_dest_evts in Hrel; eauto.
+  - eapply mo_dest_evts in Hrel; eauto.
+  - eapply rb_dest_evts in Hrel; eauto.
+Qed.
+
+(* Variable Hcomp: complete_exec ex.
+
+Lemma Hval: valid_exec ex.
+Proof. destruct Hcomp; auto. Qed. *)
+
+(** ** Extended coherence order *)
+
+(** The extended coherence order is the transitive closure of the union of
+reads-from, modification order and reads-before. It corresponds to the 
+communication relation in some other works on axiomatic memory models *)
+
+Definition eco := ((rf ex) ⊔ (mo ex) ⊔ rb)^+.
+
+(** We can rewrite [eco] as the union of read-from, modification-order and read-
+before sequenced before the reflexive closure of read-from *)
+
+Open Scope rel_notations.
+
+Ltac elim_conflicting_rw Hval :=
+  rewrite (rf_wr Hval), (mo_ww Hval), (rb_rw Hval);
+  mrewrite rw_0; kat.
+
+Ltac elim_conflicting_wr Hval :=
+  rewrite (rf_wr Hval), (mo_ww Hval), (rb_rw Hval);
+  mrewrite wr_0; kat.
+
+(** We can reformulation the [eco] relation as a relation that is not a 
+reflexive transitive closure *)
+
+Lemma eco_rfmorb_seq_rfref:
+  valid_exec ex ->
+  eco = (rf ex) ⊔ (((mo ex) ⊔ rb) ⋅ (rf ex)?).
+Proof.
+  intros Hval.
+  unfold eco.
+  apply ext_rel. apply antisym.
+  - apply itr_ind_l1.
+    + kat.
+    + assert ((mo ex)⋅(mo ex) ≦ (mo ex)) as Hmo_trans.
+      { destruct_val_exec Hval. destruct_mo_v Hmo_v.
+        destruct Hmopo as [_ [Hmotrans _]].
+        unfold "⋅" in Hmotrans. rewrite Hmotrans. ra_normalise. auto. }
+    ra_normalise. rewrite Hmo_trans. ra_normalise.
+    repeat (try (apply leq_cupx)).
+    1, 5, 7: kat.
+    (* all: upgrade_to_kat Event. *)
+    1, 2, 7: (elim_conflicting_rw Hval).
+    2, 4, 6, 8: (elim_conflicting_wr Hval).
+    all: unfold rb.
+    all: destruct_val_exec Hval.
+    1, 3: mrewrite (rf_unique _ _ Hrf_v).
+    3, 4: destruct_mo_v Hmo_v;
+          destruct Hmopo as [_ [Hmotrans _]];
+          mrewrite Hmotrans.
+    all: kat.
+  - kat.
+Qed.
+
+
+(** We can deduce from this that [eco] is acyclic *)
+
+Lemma eco_acyclic:
+  valid_exec ex ->
+  acyclic eco.
+Proof.
+  intros Hval.
+  unfold acyclic.
+  assert (eco^+ = eco). { apply ext_rel; unfold eco; kat. }
+  rewrite H.
+  rewrite (eco_rfmorb_seq_rfref Hval).
+  rewrite irreflexive_is_irreflexive.
+  ra_normalise.
+  repeat (rewrite union_inter).
+  repeat (apply leq_cupx).
+  - apply (rf_irr Hval).
+  - rewrite (rb_rw Hval).
+    rewrite refl_double.
+    rewrite capone.
+    mrewrite wr_0. ra.
+  - destruct_val_exec Hval. destruct_mo_v Hmo_v.
+    destruct Hmopo as [_ [_ Hmoirr]].
+    rewrite irreflexive_is_irreflexive in Hmoirr.
+    auto.
+  - unfold rb.
+    rewrite refl_shift; auto.
+    destruct_val_exec Hval.
+    mrewrite (rf_unique _ _ Hrf_v).
+    ra_normalise.
+    destruct_mo_v Hmo_v. destruct Hmopo as [_ [_ Hmoirr]].
+    rewrite irreflexive_is_irreflexive in Hmoirr.
+    auto.
+  - rewrite (rf_wr Hval), (mo_ww Hval).
+    rewrite refl_shift. auto.
+    mrewrite rw_0. ra_normalise.
+    auto.
+Qed.
+
+End Derived.
