rc11.v
@@ -20,478 +20,6 @@ Section RC11.
 
 Variable ex: Execution.
 
-(** * Derived relations *)
-
-(** ** Reads-before *)
-
-(** A read event [r] reads-before a write event [w] if it reads-from a write
-event sequenced before [w] by the modification order. It corresponds to the
-from-read relation in some other works on axiomatic memory models. *)
-
-Definition rb :=
-  (rf ex) ° ⋅ (mo ex).
-
-Lemma rf_wr:
-  valid_exec ex ->
-  (rf ex) ≡ [W] ⋅ (rf ex) ⋅ [R].
-Proof.
-  intros Hval.
-  destruct_val_exec Hval.
-  destruct Hrf_v as [_ [_ [Hwr _]]].
-  fold rf in Hwr. rewrite Hwr. unfold rf; intuition.
-Qed.
-
-Lemma mo_ww:
-  valid_exec ex ->
-  (mo ex) ≡ [W] ⋅ (mo ex) ⋅ [W].
-Proof.
-  intros Hval.
-  destruct_val_exec Hval.
-  destruct Hmo_v as [Hmo _].
-  fold mo in Hmo. rewrite Hmo. unfold mo; intuition.
-Qed.
-
-Lemma rb_rw:
-  valid_exec ex ->
-  rb ≡ [R] ⋅ rb ⋅ [W].
-Proof.
-  intros Hval.
-  unfold rb.
-  rewrite (mo_ww Hval).
-  rewrite (rf_wr Hval).
-  ra_normalise.
-  rewrite 2injcnv.
-  kat.
-Qed.
-
-(** In a valid execution, the sequenced-before relation is irreflexive *)
-
-Lemma sb_irr:
-  valid_exec ex ->
-  irreflexive (sb ex).
-Proof.
-  intros Hval.
-  apply irreflexive_is_irreflexive.
-  destruct_val_exec Hval.
-  destruct_sb_v Hsb_v.
-  destruct Hsb_lso as [_ [_ Hsbirr]].
-  intros x. apply Hsbirr.
-Qed.
-
-(** In a valid execution, the read-from relation is irreflexive *)
-
-Lemma rf_irr:
-  valid_exec ex ->
-  irreflexive (rf ex).
-Proof.
-  intros Hval.
-  unfold irreflexive.
-  rewrite (rf_wr Hval), refl_double, capone.
-  mrewrite rw_0. ra.
-Qed.
-
-(** In a valid execution, the modification order is irreflexive *)
-
-Lemma mo_irr:
-  valid_exec ex ->
-  irreflexive (mo ex).
-Proof.
-  intros Hval.
-  apply irreflexive_is_irreflexive.
-  intros x Hnot.
-  destruct_val_exec Hval.
-  destruct_mo_v Hmo_v.
-  destruct Hmopo as [_ [_ ?]].
-  apply (H x). auto.
-Qed.
-
-(** In a valid execution, the reads-before relation is irreflexive *)
-
-Lemma rb_irr:
-  valid_exec ex ->
-  irreflexive rb.
-Proof.
-  intros Hval.
-  unfold irreflexive.
-  rewrite (rb_rw Hval), refl_double, capone.
-  mrewrite wr_0. ra.
-Qed.
-
-
-(** In a valid_execution, two events related by read-before belong to the set of
-events of the execution *)
-
-Lemma rb_orig_evts (x y : Event):
-  valid_exec ex ->
-  rb x y ->
-  In _ (evts ex) x.
-Proof.
-  intros Hval Hrb.
-  destruct Hrb as [z Hrf Hmo].
-  simp_cnv Hrf.
-  eapply rf_dest_evts; eauto using Hval.
-Qed.
-
-Lemma rb_dest_evts (x y : Event):
-  valid_exec ex ->
-  rb x y ->
-  In _ (evts ex) y.
-Proof.
-  intros Hval Hrb.
-  destruct Hrb as [z Hrf Hmo].
-  eapply mo_dest_evts; eauto using Hval.
-Qed.
-
-(** In a valid execution, an event in the origin of read-before is a read
-event *)
-
-Lemma rb_orig_read (x y : Event):
-  valid_exec ex ->
-  rb x y ->
-  is_read x.
-Proof.
-  intros Hval Hrb.
-  destruct Hrb as [z Hrf Hmo].
-  simp_cnv Hrf.
-  eapply rf_dest_read; eauto using Hval.
-Qed.
-
-(** In a valid execution, an event in the destination of read-before is a
-write event *)
-
-Lemma rb_dest_write (x y : Event):
-  valid_exec ex ->
-  rb x y ->
-  is_write y.
-Proof.
-  intros Hval Hrb.
-  destruct Hrb as [z Hrf Hmo].
-  eapply mo_dest_write; eauto using Hval.
-Qed.
-
-(** In a valid execution, two events related by read-before affect the same
-location *)
-
-Lemma rb_same_loc (x y : Event):
-  valid_exec ex ->
-  rb x y ->
-  (get_loc x) = (get_loc y).
-Proof.
-  intros Hval Hrb.
-  destruct Hrb as [z Hrf Hmo].
-  simp_cnv Hrf.
-  apply rf_same_loc in Hrf.
-  apply mo_same_loc in Hmo.
-  congruence.
-  all: eauto using Hval.
-Qed.
-
-(** In a valid execution, two events related by read-before are different *)
-
-Lemma rb_diff (x y : Event):
-  valid_exec ex ->
-  rb x y ->
-  x <> y.
-Proof.
-  intros Hval Hrb Heq.
-  eapply rb_irr. auto.
-  split; eauto.
-Qed.
-
-(** In a valid execution, reads-before is acyclic *)
-
-Lemma rb_ac:
-  valid_exec ex ->
-  acyclic rb.
-Proof.
-  intros Hval x Hcyc.
-  rewrite tc_inv_dcmp2 in Hcyc.
-  destruct Hcyc as [y Hfirst Hcyc].
-  rewrite rtc_inv_dcmp6 in Hcyc.
-  destruct Hcyc as [Hcyc|Hcyc].
-  { simpl in Hcyc. rewrite Hcyc in Hfirst.
-    eapply (rb_irr Hval x x); try (split; simpl); intuition eauto. }
-  rewrite tc_inv_dcmp2 in Hcyc.
-  destruct Hcyc as [z Hsecond Hcyc].
-  rewrite (rb_rw Hval) in Hfirst, Hsecond.
-  apply simpl_trt_tright in Hfirst.
-  apply simpl_trt_tleft in Hsecond.
-  destruct y; intuition auto.
-Qed.
-
-(** In a valid execution the union of modification-order and reads-before is
-acyclic *)
-
-Lemma rbmo_ac:
-  valid_exec ex ->
-  acyclic (rb ⊔ (mo ex)).
-Proof.
-  intros Hval x Hcyc.
-  rewrite union_comm in Hcyc.
-  unshelve (eapply (cyc_u_of_ac_implies_cyc_seq _ _ _ _ _ _) in Hcyc).
-  - unfold acyclic. apply mo_ac. eauto.
-  - intros z1 z2 [z3 H1 H2].
-    eapply mo_trans; eauto.
-  - apply rb_ac. auto.
-  - destruct Hcyc as [y Hcyc].
-    rewrite tc_inv_dcmp2 in Hcyc.
-    destruct Hcyc as [z1 [z2 Hmo Hrb] _].
-    rewrite tc_inv_dcmp2 in Hrb.
-    destruct Hrb as [z3 Hrb _].
-    rewrite (rb_rw Hval) in Hrb.
-    apply (mo_ww Hval) in Hmo.
-    apply simpl_trt_tright in Hmo.
-    apply simpl_trt_tleft in Hrb.
-    destruct z2; simpl in Hmo, Hrb; intuition auto.
-Qed.
-
-
-(** In a valid execution, the union of sequenced-before, reads-from, 
-modification order and reads-before is irreflexive *)
-
-Lemma sbrfmorb_irr:
-  valid_exec ex ->
-  irreflexive (sb ex ⊔ rf ex ⊔ mo ex ⊔ rb).
-Proof.
-  intros Hval.
-  apply irreflexive_union.
-  apply irreflexive_union.
-  apply irreflexive_union.
-  apply (sb_irr Hval).
-  apply (rf_irr Hval).
-  apply (mo_irr Hval).
-  apply (rb_irr Hval).
-Qed.
-
-Lemma sbrf_irr:
-  valid_exec ex ->
-  irreflexive (sb ex ⊔ rf ex).
-Proof.
-  intros Hval.
-  apply irreflexive_union.
-  - auto using sb_irr.
-  - auto using rf_irr.
-Qed.
-
-Lemma rtc_sbrfmorb_in_l_aux (x y: Event):
-  valid_exec ex ->
-  (sb ex ⊔ rf ex ⊔ mo ex ⊔ rb)^* x y ->
-  (fun z1 z2 => In _ (evts ex) z2 -> In _ (evts ex) z1) x y.
-Proof.
-  intros Hval.
-  apply rtc_ind.
-  - intros z1 z2 [[[Hsb|Hrf]|Hmo]|Hrb]; intros Hin.
-    * eapply sb_orig_evts; eauto.
-    * eapply rf_orig_evts; eauto.
-    * eapply mo_orig_evts; eauto.
-    * eapply rb_orig_evts; eauto.
-  - intuition auto.
-  - intuition auto.
-Qed.
-
-Lemma rtc_sbrfmorb_in_l (x y: Event):
-  valid_exec ex ->
-  (sb ex ⊔ rf ex ⊔ mo ex ⊔ rb)^* x y ->
-  In _ (evts ex) y ->
-  In _ (evts ex) x.
-Proof.
-  intros Hval Hrel Hy. eapply rtc_sbrfmorb_in_l_aux; eauto.
-Qed.
-
-Lemma rtc_sbrfmorb_in_r_aux (x y: Event):
-  valid_exec ex ->
-  (sb ex ⊔ rf ex ⊔ mo ex ⊔ rb)^* x y ->
-  (fun z1 z2 => In _ (evts ex) z1 -> In _ (evts ex) z2) x y.
-Proof.
-  intros Hval.
-  apply rtc_ind.
-  - intros z1 z2 [[[Hsb|Hrf]|Hmo]|Hrb]; intros Hin.
-    * eapply sb_dest_evts; eauto.
-    * eapply rf_dest_evts; eauto.
-    * eapply mo_dest_evts; eauto.
-    * eapply rb_dest_evts; eauto.
-  - intuition auto.
-  - intuition auto.
-Qed.
-
-Lemma rtc_sbrfmorb_in_r (x y: Event):
-  valid_exec ex ->
-  (sb ex ⊔ rf ex ⊔ mo ex ⊔ rb)^* x y ->
-  In _ (evts ex) x ->
-  In _ (evts ex) y.
-Proof.
-  intros Hval Hrel Hy. eapply rtc_sbrfmorb_in_r_aux; eauto.
-Qed.
-
-Lemma tc_sbrfmorb_in_l_aux (x y: Event):
-  valid_exec ex ->
-  (sb ex ⊔ rf ex ⊔ mo ex ⊔ rb)^+ x y ->
-  (fun z1 z2 => In _ (evts ex) z1) x y.
-Proof.
-  intros Hval.
-  apply tc_ind.
-  - intros z1 z2 [[[Hsb|Hrf]|Hmo]|Hrb].
-    * eapply sb_orig_evts; eauto.
-    * eapply rf_orig_evts; eauto.
-    * eapply mo_orig_evts; eauto.
-    * eapply rb_orig_evts; eauto.
-  - intuition auto.
-Qed.
-
-Lemma tc_sbrfmorb_in_l (x y: Event):
-  valid_exec ex ->
-  (sb ex ⊔ rf ex ⊔ mo ex ⊔ rb)^+ x y ->
-  In _ (evts ex) x.
-Proof.
-  intros Hval Hrel. eapply tc_sbrfmorb_in_l_aux; eauto.
-Qed.
-
-Lemma tc_sbrfmorb_in_r_aux (x y: Event):
-  valid_exec ex ->
-  (sb ex ⊔ rf ex ⊔ mo ex ⊔ rb)^+ x y ->
-  (fun z1 z2 => In _ (evts ex) z2) x y.
-Proof.
-  intros Hval.
-  apply tc_ind.
-  - intros z1 z2 [[[Hsb|Hrf]|Hmo]|Hrb].
-    * eapply sb_dest_evts; eauto.
-    * eapply rf_dest_evts; eauto.
-    * eapply mo_dest_evts; eauto.
-    * eapply rb_dest_evts; eauto.
-  - intuition auto.
-Qed.
-
-Lemma tc_sbrfmorb_in_r (x y: Event):
-  valid_exec ex ->
-  (sb ex ⊔ rf ex ⊔ mo ex ⊔ rb)^+ x y ->
-  In _ (evts ex) y.
-Proof.
-  intros Hval Hrel. eapply tc_sbrfmorb_in_r_aux; eauto.
-Qed.
-
-Lemma sbrfmorb_in_l (x y: Event):
-  valid_exec ex ->
-  (sb ex ⊔ rf ex ⊔ mo ex ⊔ rb) x y ->
-  In _ (evts ex) x.
-Proof.
-  intros Hval Hrel.
-  destruct Hrel as [[[Hrel|Hrel]|Hrel]|Hrel].
-  - eapply sb_orig_evts in Hrel; eauto.
-  - eapply rf_orig_evts in Hrel; eauto.
-  - eapply mo_orig_evts in Hrel; eauto.
-  - eapply rb_orig_evts in Hrel; eauto.
-Qed.
-
-Lemma sbrfmorb_in_r (x y: Event):
-  valid_exec ex ->
-  (sb ex ⊔ rf ex ⊔ mo ex ⊔ rb) x y ->
-  In _ (evts ex) y.
-Proof.
-  intros Hval Hrel.
-  destruct Hrel as [[[Hrel|Hrel]|Hrel]|Hrel].
-  - eapply sb_dest_evts in Hrel; eauto.
-  - eapply rf_dest_evts in Hrel; eauto.
-  - eapply mo_dest_evts in Hrel; eauto.
-  - eapply rb_dest_evts in Hrel; eauto.
-Qed.
-
-(* Variable Hcomp: complete_exec ex.
-
-Lemma Hval: valid_exec ex.
-Proof. destruct Hcomp; auto. Qed. *)
-
-(** ** Extended coherence order *)
-
-(** The extended coherence order is the transitive closure of the union of
-reads-from, modification order and reads-before. It corresponds to the 
-communication relation in some other works on axiomatic memory models *)
-
-Definition eco := ((rf ex) ⊔ (mo ex) ⊔ rb)^+.
-
-(** We can rewrite [eco] as the union of read-from, modification-order and read-
-before sequenced before the reflexive closure of read-from *)
-
-Open Scope rel_notations.
-
-Ltac elim_conflicting_rw Hval :=
-  rewrite (rf_wr Hval), (mo_ww Hval), (rb_rw Hval);
-  mrewrite rw_0; kat.
-
-Ltac elim_conflicting_wr Hval :=
-  rewrite (rf_wr Hval), (mo_ww Hval), (rb_rw Hval);
-  mrewrite wr_0; kat.
-
-(** We can reformulation the [eco] relation as a relation that is not a 
-reflexive transitive closure *)
-
-Lemma eco_rfmorb_seq_rfref:
-  valid_exec ex ->
-  eco = (rf ex) ⊔ (((mo ex) ⊔ rb) ⋅ (rf ex)?).
-Proof.
-  intros Hval.
-  unfold eco.
-  apply ext_rel. apply antisym.
-  - apply itr_ind_l1.
-    + kat.
-    + assert ((mo ex)⋅(mo ex) ≦ (mo ex)) as Hmo_trans.
-      { destruct_val_exec Hval. destruct_mo_v Hmo_v.
-        destruct Hmopo as [_ [Hmotrans _]].
-        unfold "⋅" in Hmotrans. rewrite Hmotrans. ra_normalise. auto. }
-    ra_normalise. rewrite Hmo_trans. ra_normalise.
-    repeat (try (apply leq_cupx)).
-    1, 5, 7: kat.
-    (* all: upgrade_to_kat Event. *)
-    1, 2, 7: (elim_conflicting_rw Hval).
-    2, 4, 6, 8: (elim_conflicting_wr Hval).
-    all: unfold rb.
-    all: destruct_val_exec Hval.
-    1, 3: mrewrite (rf_unique _ _ Hrf_v).
-    3, 4: destruct_mo_v Hmo_v;
-          destruct Hmopo as [_ [Hmotrans _]];
-          mrewrite Hmotrans.
-    all: kat.
-  - kat.
-Qed.
-
-
-(** We can deduce from this that [eco] is acyclic *)
-
-Lemma eco_acyclic:
-  valid_exec ex ->
-  acyclic eco.
-Proof.
-  intros Hval.
-  unfold acyclic.
-  assert (eco^+ = eco). { apply ext_rel; unfold eco; kat. }
-  rewrite H.
-  rewrite (eco_rfmorb_seq_rfref Hval).
-  rewrite irreflexive_is_irreflexive.
-  ra_normalise.
-  repeat (rewrite union_inter).
-  repeat (apply leq_cupx).
-  - apply (rf_irr Hval).
-  - rewrite (rb_rw Hval).
-    rewrite refl_double.
-    rewrite capone.
-    mrewrite wr_0. ra.
-  - destruct_val_exec Hval. destruct_mo_v Hmo_v.
-    destruct Hmopo as [_ [_ Hmoirr]].
-    rewrite irreflexive_is_irreflexive in Hmoirr.
-    auto.
-  - unfold rb.
-    rewrite refl_shift; auto.
-    destruct_val_exec Hval.
-    mrewrite (rf_unique _ _ Hrf_v).
-    ra_normalise.
-    destruct_mo_v Hmo_v. destruct Hmopo as [_ [_ Hmoirr]].
-    rewrite irreflexive_is_irreflexive in Hmoirr.
-    auto.
-  - rewrite (rf_wr Hval), (mo_ww Hval).
-    rewrite refl_shift. auto.
-    mrewrite rw_0. ra_normalise.
-    auto.
-Qed.
-
 (** ** Release sequence *)
 
 (** The release sequence of a write event contains the write itself (if it is
@@ -554,7 +82,7 @@ Qed.
 (** ** SC-before *)
 
 Definition scb :=
- (sb ex) ⊔  ((res_neq_loc (sb ex)) ⋅ hb ⋅ (res_neq_loc (sb ex))) ⊔ (res_eq_loc hb) ⊔ (mo ex) ⊔  rb.
+ (sb ex) ⊔  ((res_neq_loc (sb ex)) ⋅ hb ⋅ (res_neq_loc (sb ex))) ⊔ (res_eq_loc hb) ⊔ (mo ex) ⊔  (rb ex).
 
 (** happens-before can be decomposed in a subset of happens-before included in
 SC-before, and the rest of happens-before *)
@@ -662,7 +190,7 @@ Definition psc_base :=
 occur *)
 
 Definition psc_fence :=
-  [F] ⋅ [M Sc] ⋅ (hb ⊔ (hb ⋅ eco ⋅ hb)) ⋅ [F] ⋅ [M Sc].
+  [F] ⋅ [M Sc] ⋅ (hb ⊔ (hb ⋅ (eco ex) ⋅ hb)) ⋅ [F] ⋅ [M Sc].
 
 (** ** Partial SC *)
 
@@ -681,7 +209,7 @@ patterns in executions. These patterns are detailed in proposition 1 of section
 condition *)
 
 Definition coherence :=
-  forall x, ~(hb ⋅ eco ?) x x.
+  forall x, ~(hb ⋅ (eco ex) ?) x x.
   
 
 (** In a coherent execution, [hb] is irreflexive. This means that an event
@@ -810,12 +338,12 @@ Qed.
 memory models *)
 
 Theorem coherence_is_uniproc:
-  valid_exec ex -> coherence -> irreflexive ((sb ex) ⋅ eco).
+  valid_exec ex -> coherence -> irreflexive ((sb ex) ⋅ (eco ex)).
 Proof.
   intros Hval Hco.
   apply seq_refl_incl_left with (r3 := hb).
   - unfold sb, hb. kat.
-  - rewrite (eco_rfmorb_seq_rfref Hval).
+  - rewrite (eco_rfmorb_seq_rfref _ Hval).
     unfold irreflexive.
     ra_normalise.
     repeat (rewrite union_inter).
@@ -845,7 +373,7 @@ Qed.
 adjacent in [eco]: there is no write event in between *)
 
 Definition atomicity :=
-  forall x y, ~ ((rmw ex) ⊓ (rb ⋅ (mo ex))) x y.
+  forall x y, ~ ((rmw ex) ⊓ ((rb ex) ⋅ (mo ex))) x y.
 
 (** ** SC *)
 
@@ -877,7 +405,7 @@ Definition rc11_consistent :=
 Lemma rc11_rmw_incl_rb:
   complete_exec ex ->
   rc11_consistent ->
-  rmw ex ≦ rb.
+  rmw ex ≦ (rb ex).
 Proof.
   intros Hcomp [Hco _] x y Hrmw.
   inversion Hcomp as [Hval _].
@@ -937,7 +465,7 @@ Qed.
 *)
 
 Definition sc_consistent :=
-  atomicity /\ acyclic ((sb ex) ⊔ (rf ex) ⊔ (mo ex) ⊔ rb).
+  atomicity /\ acyclic ((sb ex) ⊔ (rf ex) ⊔ (mo ex) ⊔ (rb ex)).
 
 Lemma sc_is_rc11:
   valid_exec ex ->
@@ -1000,7 +528,7 @@ Qed.
 Lemma rc11_is_sc_aux:
   valid_exec ex ->
   (forall e, In _ (evts ex) e -> (get_mode e = Sc)) ->
-  (sb ex ⊔ eco) ≦ (hb ? ⋅ scb ⋅ hb ?)^+.
+  (sb ex ⊔ (eco ex)) ≦ (hb ? ⋅ scb ⋅ hb ?)^+.
 Proof.
   intros Hval Hallsc.
   apply union_incl.
@@ -1057,7 +585,7 @@ Lemma empty_mo_ac_eco:
   valid_exec ex ->
   no_thin_air ->
   (mo ex) = empty ->
-  acyclic ((sb ex) ⊔ (rf ex) ⊔ (mo ex) ⊔ rb).
+  acyclic ((sb ex) ⊔ (rf ex) ⊔ (mo ex) ⊔ (rb ex)).
 Proof.
   intros Hval Hnoota Hmoempty x Hcyc.
   unfold rb in Hcyc. rewrite Hmoempty in Hcyc.
